theories/VLSM/Core/VLSM.v
@@ -671,10 +671,9 @@ given inputs and that they have a [valid_state] and a [valid_message].
       (l : label)
       (som : state * option message)
       (Hv : input_valid l som)
-      : exists (som' : state * option message),
+      : forall som', transition l som = som' ->
         input_valid_transition l som som'.
     Proof.
-      exists (transition l som).
       repeat split; assumption.
     Qed.
 
@@ -686,7 +685,8 @@ given inputs and that they have a [valid_state] and a [valid_message].
             input_valid_transition l som som'.
     Proof.
       split.
-      - apply input_valid_can_transition.
+      - eexists.
+        apply input_valid_can_transition; [assumption|reflexivity].
       - intros [som' Hivt].
         apply input_valid_transition_valid with som'.
         assumption.
